755/Project2/ParameterizedStack.v
@@ -6,103 +6,122 @@ Require Import Omega.
 (* 2015.10.19 *)
 
 (*************************Problem 2**********************)
-Inductive SC : Type :=
-  | Value : nat -> SC
-  | Unknown : SC.
+Inductive SC (T: Type) : Type :=
+  | Value : T -> SC T
+  | Unknown : SC T.
 
-Inductive Stack : Type :=
-  | Empty : Stack
-  | Add : SC -> Stack -> Stack.
+Inductive Stack (T: Type) : Type :=
+  | Empty : Stack T
+  | Add : T -> Stack T -> Stack T.
 
-(* 
+(*
   Preconditions: None 
-  Postconditions: n is top of resulting stack
+  Postconditions: t is top of resulting stack
   Invariants: resulting stack is same as s except for new top element
 *)
-Definition push (v: SC) (s : Stack) : Stack :=
-  Add v s.
+Definition push (T : Type) (e : T) (s : Stack T) : Stack T :=
+  Add T e s.
 
-(* 
+(*
   Preconditions: s is not empty
   Postconditions: top element removed from stack
   Invariants: resulting stack is same except for removed top element
 *)
-Definition pop (s : Stack) : Stack  :=
+Definition pop (T : Type) (s : Stack T) : Stack T  :=
   match s with
-    | Empty => Empty
-    | Add v s => s
+    | Empty => Empty T
+    | Add _ s => s
   end.
 
 (* 
   Preconditions: s is not empty
-  Postconditions: SC is top element of stack
-  Invariants: stack is unchanged
+  Postconditions: nat is top element of stack
+  Invariants: None
 *)
-Definition top (s : Stack) : SC :=
+Definition top (T: Type) (s : Stack T) : SC T :=
   match s with
-    | Empty => Unknown
-    | Add v s => v
+    | Empty => Unknown T
+    | Add n s => Value T n
   end.
 
 (* 
   Preconditions: None
   Postconditions: true if stack is empty, false otherwise
-  Invariants: stack is unchanged
+  Invariants: None
 *)
-Definition isEmpty (s : Stack) : bool :=
+Definition isEmpty (T: Type) (s : Stack T) : bool :=
   match s with
     | Empty => true
     | Add _ _ => false
   end.
 
-Fixpoint size (s : Stack) : nat :=
+Fixpoint size (T : Type) (s : Stack T) : nat :=
   match s with
     | Empty => 0
-    | Add _ s => 1 + size s
+    | Add _ s => 1 + size T s
   end.
 
-Theorem top_correct : forall n s, top (Add n s) = n.
+Theorem top_correct : forall T n s, top T (Add T n s) = Value T n.
 Proof.
   intros.
-  simpl.
   reflexivity.
 Qed.
 
-Theorem push_immediate : forall n s, top (push n s) = n.
+Theorem push_immediate : forall T n s, top T (push T n s) = Value T n.
 Proof.
   intros.
-  simpl.
   reflexivity.
 Qed.
 
-Theorem push_increase_size : forall n s, size (push n s) = 1 + size s.
+Theorem push_increase_size : forall T n s, size T (push T n s) = 1 + size T s.
 Proof.
   intros.
-  simpl.
   reflexivity.
 Qed.
 
-Theorem push_invariant : forall n s, pop (push n s) = s.
+Theorem push_invariant : forall T n s, pop T (push T n s) = s.
 Proof.
   intros.
-  simpl.
   reflexivity.
 Qed.
 
-Theorem pop_imediate : forall v s, size (pop (Add v s)) = size s.
+Theorem pop_imediate : forall T n s, size T (pop T (Add T n s)) = size T s.
 Proof.
   intros.
-  simpl.
   reflexivity.
 Qed.
 
-Theorem isEmpty_correct_true : isEmpty(Empty) = true.
+Theorem pop_invariant : forall T n s, pop T (Add T n s) = s.
+Proof.
+  intros.
+  reflexivity.
+Qed.
+
+Theorem isEmpty_correct_true : forall T, isEmpty T (Empty T) = true.
+Proof.
+  intros.
+  reflexivity.
+Qed.
+
+Theorem isEmpty_correct_false : forall T n s, isEmpty T (Add T n s) = false.
+Proof.
+  intros.
+  reflexivity.
+Qed.
+
+(* Two pops on two pushes is always safe because no matter what is pushed,
+two items will be on the stack before removing those two elements with the pops.
+Therefore, the precondition of not popping on an emtpy stack will be avoided. *)
+Example pop_push_safe : forall T x y, (pop T (pop T (push T x (push T y (Empty T))))) = Empty T.
 Proof.
   reflexivity.
 Qed.
 
-Theorem isEmpty_correct_false : forall n s, isEmpty(Add n s) = false.
+(* Two pops on a single push will not crash. However, it is not safe because 
+pushing a single item and then popping twice leads to violating the precondition 
+for pop that you don't pop on an empty stack. Although you'll get an empty stack
+back, no pop was actually executed because there were no items to pop.*)
+Example pop_push_unsafe : forall T x, (pop T (pop T (push T x (Empty T)))) = Empty T.
 Proof.
-  intros.
   reflexivity.
 Qed.
